coq/cclc/clc_inversion.v
@@ -75,3 +75,88 @@ Proof.
   move=> /pi_inv[t[i[tyA tyB]]] tyL.
   apply: lam_invX; eauto.
 Qed.
+
+Lemma it_invX Γ1 A :
+  Γ1 ⊢ It : A -> A <: Unit -> Γ1 |> U.
+Proof.
+  move e:(It)=>m tp. elim:tp e=>//{Γ1 m A}.
+  move=>Γ A B m s i sb1 tym ihm tyB ihB e sb2; subst.
+  apply: ihm; eauto.
+  apply: sub_trans; eauto.
+Qed.
+
+Lemma it_inv Γ1 : Γ1 ⊢ It : Unit -> Γ1 |> U.
+Proof. move=>ty. apply: it_invX; eauto. Qed.
+
+Lemma sigma_inv Γ A B s r t x :
+  Γ ⊢ Sigma A B s r t : x ->
+  exists Γ1 Γ2 t i,
+    Γ1 ∘ Γ2 => Γ /\
+    Γ1 ⊢ A : s @ i /\ [A :{s} Γ2] ⊢ B : t @ i.
+Proof.
+  move e:(Sigma A B s r t)=>m ty. 
+  elim: ty A B s r t e=>//{Γ x m}.
+  move=>Γ A B s r t i mrg k 
+    tyA ihA tyB ihB A0 B0 s0 r0 t0 [e1 e2 e3 e4 e5]; subst.
+  exists Γ. exists Γ. 
+  exists r. exists i. firstorder.
+  by apply: merge_pure.
+Qed.
+
+Lemma pair_invX Γ m n C :
+  Γ ⊢ Pair m n : C ->
+  forall A B s r t x l,
+    C <: Sigma A B s r t ->
+    [Γ] ⊢ Sigma A B s r t : x @ l ->
+    exists Γ1 Γ2,
+      Γ1 |> s /\ 
+      Γ2 |> r /\
+      Γ1 ∘ Γ2 => Γ /\
+      Γ1 ⊢ m : A /\ Γ2 ⊢ n : B.[m/].
+Proof.
+  move e:(Pair m n)=>v tp. elim: tp m n e=>//{Γ v C}.
+  move=>Γ1 Γ2 Γ A B m n s r t i k1 k2 mrg.
+  move=>/sigma_inv[G1[G2[t0[i0[mrg0[tyA tyB]]]]]].
+  move=>_ tym _ tyn _ m0 n0 [e1 e2] A0 B0 s1 r1 t1 x l.
+  move=>/sub_sigma_inv[sbA[sbB[e3[e4 e5]]]]; subst.
+  move=>/sigma_inv[G3[G4[t2[i1[mrg1[tyA0 tyB0]]]]]].
+  { exists Γ1. exists Γ2.
+    have[_[e1 e2]]:=merge_re_re mrg.
+    have[_[e3 e4]]:=merge_re_re mrg1.
+    rewrite<-re_invo in e3.
+    rewrite<-re_invo in e4.
+    have[k3 k4]:=merge_pure_inv mrg1 (re_pure _).
+    repeat split; eauto.
+    apply: clc_conv; eauto.
+    rewrite e1.
+    rewrite<-e3.
+    rewrite<-pure_re; eauto.
+    apply: clc_conv.
+    apply: sub_subst; eauto.
+    eauto.
+    destruct s1; simpl in tyB0.
+    { have mrg2:[G4] ∘ Γ1 => [Γ2].
+      rewrite e4 e2 (pure_re k1) e1.
+      apply: merge_re_id.
+      have {}tym:Γ1 ⊢ m : A0.
+      apply:clc_conv; eauto.
+      rewrite e1. rewrite<-e3. rewrite<-pure_re; eauto.
+      have:=substitution tyB0 k1 mrg2 tym. 
+      asimpl; eauto. }
+    { have:=substitutionN tyB0 tym.
+      rewrite e4. by rewrite<-e2. } }
+  move=>Γ A B m s i sb1 tym ihm tyB ihB 
+    m0 n e A0 B0 s0 r t x l sb2 tyS; subst.
+  { apply: ihm; eauto.
+    apply: sub_trans; eauto. }
+Qed.
+
+Lemma pair_inv Γ m n A B s r t x i :
+  Γ ⊢ Pair m n : Sigma A B s r t ->
+  [Γ] ⊢ Sigma A B s r t : x @ i ->
+  exists Γ1 Γ2,
+    Γ1 |> s /\ 
+    Γ2 |> r /\
+    Γ1 ∘ Γ2 => Γ /\
+    Γ1 ⊢ m : A /\ Γ2 ⊢ n : B.[m/].
+Proof. move=>tyP tyS. apply: pair_invX; eauto. Qed.
